QR/ZK.ec
@@ -4,7 +4,7 @@ require import AllCore DBool Bool List Distr Int Aux DJoin.
 require import  Basics Sim1Property.
 
 import OSS.
-import OMZK.
+(* import OMZK. *)
 
 clone import  StatisticalZK with op negl <- 0%r.
 
@@ -16,8 +16,9 @@ section.
 
 
 
-declare module V <: RewMaliciousVerifier{-HP, -OMZK.MW.IFB.IM.W, -OMZK.MW.IFB.DW}.
-declare module D <: ZKDistinguisher{-OMZK.MW.IFB.IM.W, -OMZK.MW.IFB.DW}.
+declare module V <: RewMaliciousVerifier{-HP}.
+declare module D <: ZKDistinguisher{-HP}.
+
 
 
 declare axiom Sim1_run_ll : forall (V0 <: RewMaliciousVerifier), islossless V0.challenge => islossless V0.summitup => islossless Sim1(V0).run.
@@ -25,6 +26,8 @@ declare axiom D_guess_prop : equiv[ D.guess ~ D.guess : ={glob V, arg} ==> ={res
 declare axiom V_summitup_ll : islossless V.summitup. 
 declare axiom V_challenge_ll : islossless V.challenge.
 declare axiom D_guess_ll : islossless D.guess.
+declare axiom P_response_ll : islossless HP.response.
+declare axiom P_commitment_ll : islossless HP.commitment.
 
 
 declare axiom rewindable_V_plus : 
@@ -41,20 +44,21 @@ declare axiom rewindable_V_plus :
 lemma qr_statistical_zk stat wit &m:
         IsSqRoot stat  wit  => unit stat =>
         let real_prob = Pr[ZKReal(HP, V, D).run(stat, wit) @ &m : res] in
-        let ideal_prob = Pr[ZKIdeal(Simulator(Sim1), V, D).run(stat, wit) @ &m : res] in
-          `|real_prob - ideal_prob| <= 2%r * (1%r / 2%r) ^ n.
+        let ideal_prob = Pr[ZKIdeal(Simulator'(Sim1), V, D).run(stat, wit) @ &m : res] in
+          `|ideal_prob - real_prob| <= 2%r * (1%r / 2%r) ^ n.
 proof.
 progress.
-apply (statistical_zk HP Sim1  V D _ _ _ _ _ _ _ _ stat wit  
-  (1%r/2%r) &m);auto. apply Sim1_run_ll. apply V_summitup_ll. apply V_challenge_ll. apply D_guess_ll.
+apply (statistical_zk HP Sim1  V D _ _ _ _ _ _ _ _ _ _ stat wit  
+  (1%r/2%r) &m _ _);auto. apply Sim1_run_ll. apply V_summitup_ll. apply V_challenge_ll. 
+apply P_response_ll. apply P_commitment_ll.
+apply D_guess_ll. apply D_guess_prop.
 apply rewindable_V_plus. 
-
 apply (sim1_rew_ph V). 
  apply V_summitup_ll. apply V_challenge_ll.  apply (rewindable_A_plus V). apply rewindable_V_plus.
 progress. 
 rewrite (sim1_prop V D _ _  _ _ _  p w  _ ).  apply (rewindable_A_plus V).
  exists f. split. auto. auto.
-auto. auto.   auto.  auto. auto. apply D_guess_prop.
+auto. auto.   auto.  auto. auto. 
 rewrite (sim1assc V D _ _ _ _ &m stat  wit). apply (rewindable_A_plus V).
 apply rewindable_V_plus.
 apply V_summitup_ll.
